pulse/src/checker/Pulse.Typing.Util.fsti
@@ -31,13 +31,6 @@ val check_equiv_now_nosmt (g:env) (t1 t2 : term)
 val check_equiv_now_nosmt_unfold (g:env) (t1 t2 : term)
   : Tac (option (squash (equiv_token g t1 t2)) & issues)
 
-(* Like check_equiv_now, but disallows unfolding.
-   Produces structural arg-level guards without looking
-   through type abbreviations. Useful for slprop comparisons
-   where the abstraction level should be preserved. *)
-val check_equiv_now_nounfold (g:env) (t1 t2 : term)
-  : Tac (option (squash (equiv_token g t1 t2)) & issues)
-
 (* Like T.universe_of, but will make sure to not delay any VC. *)
 val universe_of_now : g:env -> e:term ->
   Tac (option (u:universe{typing_token g e (E_Total, pack_ln (Reflection.V2.Tv_Type u))}) & issues)
